WIP: interpreting models

LeanSts/SMT/Model.lean
@@ -1,5 +1,5 @@
-import LeanSts.SMT.Main
 import Lean
+import Auto
 
 abbrev Name := Lean.Name
 abbrev UninterpretedValue := Name
@@ -9,24 +9,64 @@ structure FiniteUinterpretedSort where
   size : Nat
   /-- The elements are assumed to be distinct. -/
   elements : Array UninterpretedValue
+deriving BEq, Hashable
+
+instance : ToString FiniteUinterpretedSort where
+  toString s := s!"uninterpreted sort {s.name} {s.elements}"
 
 structure InterpretedSort where
   name : Name
-  interpretation : Type
+  -- interpretation : Type
+deriving BEq, Hashable
 
-def boolSortI : InterpretedSort := { name := `Bool, interpretation := Bool }
-def intSortI : InterpretedSort := { name := `Int, interpretation := Int }
+instance : ToString InterpretedSort where
+  toString s := s!"interpreted sort {s.name}"
+
+def boolSortI : InterpretedSort := { name := `Bool }
+def intSortI : InterpretedSort := { name := `Int }
+
+def builtinInterpretedSorts : Lean.HashMap Name InterpretedSort :=
+  Lean.HashMap.ofList [(`Bool, boolSortI), (`Int, intSortI)]
+
+def InterpretedSort.interpretation (s : InterpretedSort) : Type :=
+  match s.name with
+  | `Bool => Bool
+  | `Int => Int
+  | _ => Unit
+
+/- FIXME: I don't know how to write this without tactics. -/
+def InterpretedSort.valToString {s : InterpretedSort} (val : s.interpretation) : String := by
+  unfold interpretation at val
+  split at val <;> exact (toString val)
+
+instance : BEq InterpretedSort where
+  beq s₁ s₂ := s₁.name == s₂.name
+
+instance : Hashable InterpretedSort where
+  hash s := (`InterpretedSort ++ s.name).hash
 
 inductive FirstOrderSort
   | Interpreted (s : InterpretedSort)
   | Uninterpreted (s : FiniteUinterpretedSort)
+deriving BEq, Hashable
 
-def FirstOrderSort.valueType : FirstOrderSort → Type
-  | FirstOrderSort.Interpreted s => s.interpretation
-  | FirstOrderSort.Uninterpreted _ => UninterpretedValue
+instance : ToString FirstOrderSort where
+  toString
+    | FirstOrderSort.Interpreted s => toString s
+    | FirstOrderSort.Uninterpreted s => toString s
 
-def FirstOrderSort.valueTypeArray : Array FirstOrderSort → Array Type
-  | xs => xs.map (λ s => s.valueType)
+def FirstOrderSort.name : FirstOrderSort → Name
+  | FirstOrderSort.Interpreted s => s.name
+  | FirstOrderSort.Uninterpreted s => s.name
+
+inductive FirstOrderValue where
+  | Interpreted (s : InterpretedSort) (val : s.interpretation)
+  | Uninterpreted (s : FiniteUinterpretedSort) (val : UninterpretedValue)
+
+instance : ToString FirstOrderValue where
+  toString
+    | FirstOrderValue.Interpreted s val => s.valToString val
+    | FirstOrderValue.Uninterpreted _ val => toString val
 
 def boolSort : FirstOrderSort := FirstOrderSort.Interpreted boolSortI
 def intSort : FirstOrderSort := FirstOrderSort.Interpreted intSortI
@@ -34,20 +74,39 @@ def intSort : FirstOrderSort := FirstOrderSort.Interpreted intSortI
 structure ConstantDecl where
   name : Name
   sort : FirstOrderSort
+deriving BEq, Hashable
+
+instance : ToString ConstantDecl where
+  toString c := s!"constant {c.name} : {c.sort}"
 
 structure RelationDecl where
   name : Name
   domain : Array FirstOrderSort
+deriving BEq, Hashable
+
+instance : ToString RelationDecl where
+  toString r := s!"relation {r.name} : {r.domain}"
 
 structure FunctionDecl where
   name : Name
   domain : Array FirstOrderSort
   range : FirstOrderSort
+deriving BEq, Hashable
+
+instance : ToString FunctionDecl where
+  toString f := s!"function {f.name} : {f.domain} → {f.range}"
 
 inductive Declaration where
   | Constant (c : ConstantDecl)
   | Relation (r : RelationDecl)
   | Function (f : FunctionDecl)
+deriving BEq, Hashable
+
+instance : ToString Declaration where
+  toString
+    | Declaration.Constant c => toString c
+    | Declaration.Relation r => toString r
+    | Declaration.Function f => toString f
 
 def Declaration.name : Declaration → Name
   | Declaration.Constant c => c.name
@@ -74,49 +133,148 @@ structure Signature where
   relations : Array RelationDecl
   functions : Array FunctionDecl
 
-structure ExplicitInterpretation (sig : Signature) where
-  interp :
-    (d : Declaration) → -- TODO: `d` should be in `sig`
-    {dom : Array Type // dom = FirstOrderSort.valueTypeArray d.domain} →
-    {val : Type // val = FirstOrderSort.valueType d.range}
+instance : Inhabited Signature := ⟨{ constants := #[], relations := #[], functions := #[] }⟩
+
+abbrev ExplicitInterpretation := Lean.HashMap Declaration (Array FirstOrderValue × FirstOrderValue)
 
 structure FirstOrderStructure where
   /-- Also called universes. -/
   domains : Array FirstOrderSort
   signature : Signature
-  interp : ExplicitInterpretation signature
+  interp : ExplicitInterpretation
 
+open Lean hiding Declaration
 
-set_option trace.smt true
-set_option trace.smt.solve true
-set_option trace.smt.reconstruct.proof true
+def FirstOrderStructure.findSort (s : FirstOrderStructure) (name : Lean.Name) : MetaM FirstOrderSort :=
+  match s.domains.find? (fun s => s.name == name) with
+  | some sort => return sort
+  | none => throwError s!"sort {name} used but not previously declared!"
 
-set_option trace.sauto true
-set_option sauto.smt.solver "z3"
+def FirstOrderStructure.findDecl (s : FirstOrderStructure) (name : Lean.Name) : MetaM Declaration :=
+  match s.signature.constants.find? (fun c => c.name == name) with
+  | some c => return Declaration.Constant c
+  | none => match s.signature.relations.find? (fun r => r.name == name) with
+    | some r => return Declaration.Relation r
+    | none => match s.signature.functions.find? (fun f => f.name == name) with
+      | some f => return Declaration.Function f
+      | none => throwError s!"{name} provided an interpretation for, but not previously declared!"
 
-theorem model1 {a : Type} (rel : a → a → Prop) (f : a → Int) (s1 s2 : a) :
-  rel s1 s2 → rel s2 s1 ∨ f s1 = f s2 := by
-  sauto
+instance : Inhabited FirstOrderStructure := ⟨{ domains := #[], signature := default, interp := default }⟩
 
--- TRY:
--- (check-sat-using (then macro-finder smt))
+open Auto.Parser.SMTSexp
+abbrev Sexpr := Auto.Parser.SMTSexp.Sexp
 
-/-
-    (
-    (sort Bool (true false))
-    (sort Int ())
-    (sort a (a0 a1))
-    (function f (a) Int)
-    (interpret f (a0) -1)
-    (interpret f (a1) 0)
-    (relation rel (a a))
-    (interpret rel (a0 a0) false)
-    (interpret rel (a0 a1) false)
-    (interpret rel (a1 a0) true)
-    (interpret rel (a1 a1) false)
-    (constant s1 a)
-    (interpret s1 () a1)
-    (constant s2 a)
-    (interpret s2 () a0)
+partial def extractInstructions (e : Sexpr) (depth : Int := 0): MetaM (List Sexpr) := do
+  match e with
+  | .atom _ => throwError s!"malformed model: unexpected atom at depth {depth}"
+  | .app xs =>
+      let mut instructions : List Sexpr:= if depth == 1 then [e] else []
+      if depth == 0 then
+        for x in xs do
+          instructions := instructions ++ (← extractInstructions x (depth + 1))
+      return instructions
+
+def findSortWithName (name : Lean.Name) (struct : FirstOrderStructure) : MetaM FirstOrderSort :=
+  match struct.domains.find? (fun s => s.name == name) with
+  | some sort => return sort
+  | none => throwError s!"sort {name} used but not previously declared!"
+
+def findSortsArray (names : Array Sexp) (struct : FirstOrderStructure) : MetaM (Array FirstOrderSort) := do
+  let mut sorts : Array FirstOrderSort := #[]
+  for dom in names do
+    match dom with
+    | .atom (.symb domName) => sorts := sorts.push (← findSortWithName (Name.mkSimple domName) struct)
+    | _ => throwError s!"malformed domain: {dom}"
+  return sorts
+
+def getValueOfSort (val : Sexp) (sort : FirstOrderSort) : MetaM FirstOrderValue := do
+  match sort with
+  | FirstOrderSort.Interpreted s => do
+    match s.name with
+    | `Bool => match val with
+      | .atom (.symb "true") => return FirstOrderValue.Interpreted boolSortI true
+      | .atom (.symb "false") => return FirstOrderValue.Interpreted boolSortI false
+      | _ => throwError s!"expected a boolean value, but got {val}"
+    | `Int => match val with
+      | .atom (.nat n) => return FirstOrderValue.Interpreted intSortI (Int.ofNat n)
+      | .atom (.symb i) => return FirstOrderValue.Interpreted intSortI i.toInt!
+      | _ => throwError s!"expected an integer value, but got {val}"
+    | _ => throwError s!"unsupported interpreted sort: {s}"
+  | FirstOrderSort.Uninterpreted s => do
+    match val with
+    | .atom (.symb valName) => return FirstOrderValue.Uninterpreted s (Name.mkSimple valName)
+    | _ => throwError s!"expected an uninterpreted value, but got {val}"
+
+def getValueArray (vals : Array Sexp) (sorts : Array FirstOrderSort) : MetaM (Array FirstOrderValue) := do
+  let mut values : Array FirstOrderValue := #[]
+  for (val, sort) in Array.zip vals sorts do
+    values := values.push (← getValueOfSort val sort)
+  return values
+
+def parseInstruction (inst : Sexpr) (struct : FirstOrderStructure): MetaM (FirstOrderStructure) := do
+  let mut struct := struct
+  match inst with
+  -- (|sort| |Bool| (|true| |false|)),
+  -- (|sort| |a| (|a0| |a1|)),
+  | .app #[(.atom (.symb "sort")), (.atom (.symb sortName)), (.app els)] => do
+    let sortName := Name.mkSimple sortName
+    let sort: FirstOrderSort ← (match builtinInterpretedSorts.find? sortName with
+    | some sortI => return .Interpreted sortI
+    | none => do
+      let mut elems : Array UninterpretedValue := #[]
+      for elem in els do
+        match elem with
+        | .atom (.symb elemName) => elems := elems.push (Name.mkSimple elemName)
+        | _ => throwError s!"malformed element: {elem}"
+      return .Uninterpreted { name := sortName, size := elems.size, elements := elems }
     )
--/
+    trace[sauto] s!"{sort}"
+    struct := { struct with domains := struct.domains.push sort }
+
+  -- (|constant| |s1| |a|),
+  | .app #[(.atom (.symb "constant")), (.atom (.symb constName)), (.atom (.symb sortName))] => do
+    let constName := Name.mkSimple constName
+    let sortName := Name.mkSimple sortName
+    let sort ← findSortWithName sortName struct
+    let decl: ConstantDecl := { name := constName, sort := sort }
+    trace[sauto] s!"{decl}"
+    struct := { struct with signature := { struct.signature with constants := struct.signature.constants.push decl } }
+
+  -- (|relation| |rel| (|a| |a|)),
+  | .app #[(.atom (.symb "relation")), (.atom (.symb relName)), (.app doms)] => do
+    let relName := Name.mkSimple relName
+    let doms ← findSortsArray doms struct
+    let decl: RelationDecl := { name := relName, domain := doms }
+    trace[sauto] s!"{decl}"
+    struct := { struct with signature := { struct.signature with relations := struct.signature.relations.push decl } }
+
+  -- (|function| |f| (|a|) |Int|),
+  | .app #[(.atom (.symb "function")), (.atom (.symb funName)), (.app doms), (.atom (.symb range))] => do
+    let funName := Name.mkSimple funName
+    let doms ← findSortsArray doms struct
+    let range ← findSortWithName (Name.mkSimple range) struct
+    let decl: FunctionDecl := { name := funName, domain := doms, range := range }
+    trace[sauto] s!"{decl}"
+    struct := { struct with signature := { struct.signature with functions := struct.signature.functions.push decl } }
+
+  -- (|interpret| |rel| (|a0| |a0|) |false|)
+  -- (|interpret| |f| (|a0|) |-1|)
+  -- (|interpret| |f| (|a1|) 0)
+  | .app #[(.atom (.symb "interpret")), (.atom (.symb declName)), (.app args), val] => do
+    let declName := Name.mkSimple declName
+    let decl ← struct.findDecl declName
+    let args ← getValueArray args decl.domain
+    let val ← getValueOfSort val decl.range
+    trace[sauto] s!"interpret {declName} {args} {val}"
+    struct := { struct with interp := struct.interp.insert decl (args, val) }
+
+  | _ => throwError s!"(parseInstruction) malformed instruction: {inst}"
+  return struct
+
+def parseModel (model : Sexpr) : MetaM Unit := do
+  let mut struct : FirstOrderStructure := default
+  let instructions ← extractInstructions model
+  trace[sauto] "instructions: {instructions}"
+  for inst in instructions do
+    struct ← parseInstruction inst struct
+  return ()
